more proofs of bounds and Pack25519

Libs/Fun_Decidable.v
@@ -11,27 +11,47 @@ Context {T:Type} (n:Z). (* (Hn : 0 <= n). *)
 
 Definition dec_proof_fun (n a  : Z) : nat := Z.to_nat (a - n).
 
-Function sub_fn_rev_1 (f:Z -> T -> T) (a:Z) (t: T) {measure (dec_proof_fun n) a} : T :=
-  if (a <=? n)
-    then t
-    else
-      let prev := sub_fn_rev_1 f (a - 1) t in 
-        f (a - 1) prev.
-Proof. intros. apply Z2Nat.inj_lt ; rewrite Z.leb_gt in teq; omega. Defined.
 
-
-Function sub_fn_rev_2 (f:Z -> T -> T -> T) (a:Z) (m t: T) {measure (dec_proof_fun n) a} : T :=
+Function sub_fn_rev (f:Z -> T -> T -> T) (a:Z) (m t: T) {measure (dec_proof_fun n) a} : T :=
   if (a <=? n)
     then m
     else
-      let prev := sub_fn_rev_2 f (a - 1) m t in 
+      let prev := sub_fn_rev f (a - 1) m t in 
         f (a - 1) prev t.
 Proof. intros. apply Z2Nat.inj_lt ; rewrite Z.leb_gt in teq; omega. Defined.
+
+Lemma sub_fn_rev_1 : forall (f: Z -> T -> T -> T) (m t:T),
+  sub_fn_rev f n m t = m.
+Proof. intros. rewrite sub_fn_rev_equation ; rewrite Z.leb_refl ; reflexivity. Qed.
+
+Lemma sub_fn_rev_n : forall (a:Z) (f: Z -> T -> T -> T) (m t:T),
+  n < a ->
+  sub_fn_rev f a m t = f (a - 1) (sub_fn_rev f (a - 1) m t) t.
+Proof. intros. rewrite sub_fn_rev_equation. replace (a <=? n) with false. reflexivity.
+symmetry ; apply Z.leb_gt ; assumption. Qed.
+
+Function sub_fn_rev_s (f:Z -> T -> T) (a:Z) (t: T) {measure (dec_proof_fun n) a} : T :=
+  if (a <=? n)
+    then t
+    else
+      let prev := sub_fn_rev_s f (a - 1) t in 
+        f (a - 1) prev.
+Proof. intros. apply Z2Nat.inj_lt ; rewrite Z.leb_gt in teq; omega. Defined.
+
+Lemma sub_fn_rev_s_1 : forall (f: Z -> T -> T) (t:T),
+  sub_fn_rev_s f n t = t.
+Proof. intros. rewrite sub_fn_rev_s_equation ; rewrite Z.leb_refl ; reflexivity. Qed.
+
+Lemma sub_fn_rev_s_n : forall (a:Z) (f: Z -> T -> T) (t:T),
+  n < a ->
+  sub_fn_rev_s f a t = f (a - 1) (sub_fn_rev_s f (a - 1) t).
+Proof. intros. rewrite sub_fn_rev_s_equation. replace (a <=? n) with false. reflexivity.
+symmetry ; apply Z.leb_gt ; assumption. Qed.
 
 End fun_rec.
 
 
-Section fun_rec_denote_1.
+Section fun_rec_denote_s.
 
 Context {T:Type}.
 Context {U:Type}.
@@ -39,15 +59,15 @@ Context (t_inst : @Decidable T U).
 Context (f_inst : @Decidable (Z -> T -> T) (Z -> U -> U)).
 Context (f_t : forall env (z:Z) (f: Z -> T -> T) (t:T), denote env (f z t) = (denote env f) z (denote env t)).
 
-Inductive fun_rec_dec_1 :=
-  | Fun_n : Z -> Z -> (Z -> T -> T) -> T -> fun_rec_dec_1.
+Inductive fun_rec_dec_s :=
+  | Fun_n : Z -> Z -> (Z -> T -> T) -> T -> fun_rec_dec_s.
 
-Definition fun_rec_denote env (f:fun_rec_dec_1) : (U) := match f with
-  | Fun_n n z f' t => sub_fn_rev_1 n (denote env f') z (denote env t)
+Definition fun_rec_denote env (f:fun_rec_dec_s) : (U) := match f with
+  | Fun_n n z f' t => sub_fn_rev_s n (denote env f') z (denote env t)
   end.
 
-Definition fun_rec_denote_full env (f:fun_rec_dec_1) : (U) := match f with
-  | Fun_n n z f' t => denote env (sub_fn_rev_1 n f' z t)
+Definition fun_rec_denote_full env (f:fun_rec_dec_s) : (U) := match f with
+  | Fun_n n z f' t => denote env (sub_fn_rev_s n f' z t)
   end.
 
 Lemma fun_rec_denote_full_impl : forall env l, fun_rec_denote env l = fun_rec_denote_full env l.
@@ -55,7 +75,7 @@ Proof.
 intros env.
 destruct l as [n z f t].
 simpl.
-rewrite sub_fn_rev_1_equation ; symmetry ; rewrite sub_fn_rev_1_equation ; symmetry.
+rewrite sub_fn_rev_s_equation ; symmetry ; rewrite sub_fn_rev_s_equation ; symmetry.
 destruct (z <=? n) eqn:?.
 reflexivity.
 rewrite Z.leb_gt in Heqb.
@@ -65,7 +85,7 @@ match goal with
 end.
 2: omega.
 intros.
-rewrite sub_fn_rev_1_equation ; symmetry ; rewrite sub_fn_rev_1_equation ; symmetry.
+rewrite sub_fn_rev_s_equation ; symmetry ; rewrite sub_fn_rev_s_equation ; symmetry.
 destruct (x - 1 <=? n) eqn:?.
 rewrite f_t ; reflexivity.
 rewrite Z.leb_gt in Heqb0.
@@ -75,8 +95,8 @@ apply H.
 omega.
 Qed.
 
-Definition fun_rec_decide (l l' : fun_rec_dec_1) : bool := match l, l' with
-  | Fun_n n z f t, Fun_n n' z' f' t' => decide (sub_fn_rev_1 n f z t) (sub_fn_rev_1 n' f' z' t')
+Definition fun_rec_decide (l l' : fun_rec_dec_s) : bool := match l, l' with
+  | Fun_n n z f t, Fun_n n' z' f' t' => decide (sub_fn_rev_s n f z t) (sub_fn_rev_s n' f' z' t')
   end.
 
 Lemma fun_rec_decide_impl : forall env l l',
@@ -93,6 +113,6 @@ Proof.
   assumption.
 Qed.
 
-End fun_rec_denote_1.
+End fun_rec_denote_s.
 
 Close Scope Z.
