Low/Reduce_by_P_compose_1.v
@@ -27,8 +27,8 @@ Qed.
 
 Local Lemma sub_fn_rev_s_sub_step_1_ind_Zlength : forall a m t,
   0 <= a < Zlength m ->
-  Zlength (sub_fn_rev sub_step_1 a m t) = Zlength m ->
-  Zlength (sub_fn_rev sub_step_1 (a+1) m t) = Zlength m.
+  Zlength (sub_fn_rev 1 sub_step_1 a m t) = Zlength m ->
+  Zlength (sub_fn_rev 1 sub_step_1 (a+1) m t) = Zlength m.
 Proof.
   intros i m t Ham Hind.
   rewrite sub_fn_rev_equation.
@@ -43,7 +43,7 @@ Qed.
 Lemma sub_fn_rev_s_sub_step_1_Zlength : forall a m t,
   0 < a < 16 ->
   Zlength m = 16 ->
-  Zlength (sub_fn_rev sub_step_1 a m t) = Zlength m.
+  Zlength (sub_fn_rev 1 sub_step_1 a m t) = Zlength m.
 Proof.
   intros.
   pattern a.
@@ -64,8 +64,8 @@ Local Lemma sub_fn_rev_s_sub_step_1_ind_bound : forall a m t,
   0 < a < 16 ->
   Zlength m = 16 ->
   Forall (fun x => 0 <= x < 2 ^ 16) t ->
-  Forall (fun x => -2^16 + 1 <= x < 1) (take (Z.to_nat a) (sub_fn_rev sub_step_1 a m t)) ->
-  Forall (fun x => -2^16 + 1 <= x < 1) (take (Z.to_nat (a + 1)) (sub_fn_rev sub_step_1 (a + 1) m t)).
+  Forall (fun x => -2^16 + 1 <= x < 1) (take (Z.to_nat a) (sub_fn_rev 1 sub_step_1 a m t)) ->
+  Forall (fun x => -2^16 + 1 <= x < 1) (take (Z.to_nat (a + 1)) (sub_fn_rev 1 sub_step_1 (a + 1) m t)).
 Proof.
   intros i m t Ham Hm Hbm Hind.
   rewrite sub_fn_rev_equation.
@@ -74,7 +74,7 @@ Proof.
   replace ( i + 1 - 1) with i by omega.
   rewrite -(take_cons_Zlength _ _ 0).
   2: rewrite sub_step_1_Zlength sub_fn_rev_s_sub_step_1_Zlength; omega.
-  remember (sub_fn_rev sub_step_1 i m t) as m'.
+  remember (sub_fn_rev 1 sub_step_1 i m t) as m'.
   apply Forall_app_2.
   rewrite /sub_step_1.
   rewrite (upd_nth_alter _ (fun x => (subst_0xffff (nth (Z.to_nat i) t 0)))).
@@ -101,11 +101,11 @@ Lemma sub_fn_rev_s_sub_step_1_bound : forall i m t,
   0 < i < Zlength m ->
   Forall (fun x => 0 <= x < 2 ^ 16) t ->
   Forall (λ a : ℤ, - 2 ^ 16 + 1 ≤ a ∧ a < 1) (take (Z.to_nat 1) m) ->
-  Forall (fun x => -2^16 + 1 <= x < 1) (take (Z.to_nat i) (sub_fn_rev sub_step_1 i m t)).
+  Forall (fun x => -2^16 + 1 <= x < 1) (take (Z.to_nat i) (sub_fn_rev 1 sub_step_1 i m t)).
 Proof.
 intros.
-change(Forall (fun x => -2^16 + 1 <= x < 1) (take (Z.to_nat i) (sub_fn_rev sub_step_1 i m t))) with
-  ((fun x => Forall (fun a => -2^16 + 1 <= a < 1) (take (Z.to_nat x) (sub_fn_rev sub_step_1 x m t))) i).
+change(Forall (fun x => -2^16 + 1 <= x < 1) (take (Z.to_nat i) (sub_fn_rev 1 sub_step_1 i m t))) with
+  ((fun x => Forall (fun a => -2^16 + 1 <= a < 1) (take (Z.to_nat x) (sub_fn_rev 1 sub_step_1 x m t))) i).
 apply P016_impl ; try omega.
 rewrite sub_fn_rev_1; assumption.
 intros ; apply sub_fn_rev_s_sub_step_1_ind_bound ; try omega ; try assumption.
