Low/Reduce_by_P_compose_2b.v
@@ -1,0 +1,111 @@
+From Tweetnacl Require Import Libs.Export.
+From Tweetnacl Require Import ListsOp.Export.
+From Tweetnacl Require Import Low.Reduce_by_P_compose_step.
+From Tweetnacl Require Import Low.Reduce_by_P_compose_1.
+From Tweetnacl Require Import Low.Reduce_by_P_compose_2.
+From Tweetnacl Require Import Low.Reduce_by_P_compose.
+From stdpp Require Import prelude.
+Require Import Recdef.
+Require Import ssreflect.
+Open Scope Z.
+
+
+Lemma bound_a_subst_step_2 : forall a m,
+  0 < a < 15 ->
+  Zlength m = 16 ->
+  Forall (fun x => -2^16 < x <= 0) (take 15 m) ->
+  - 2 ^ 16 ≤ nth (Z.to_nat a) (sub_fn_rev_s 1 sub_step_2 (a + 1) m) 0 ∧ nth (Z.to_nat a) (sub_fn_rev_s 1 sub_step_2 (a + 1) m) 0 ≤ 0.
+Proof.
+intros.
+  rewrite sub_fn_rev_s_n.
+  2: omega.
+  remember (sub_fn_rev_s 1 sub_step_2 (a + 1 - 1) m) as m'.
+  replace (a + 1 - 1) with a by omega.
+  rewrite /sub_step_2.
+  rewrite upd_nth_diff_Zlength.
+  4: intro Ha; apply (f_equal Z.of_nat) in Ha ; repeat rewrite Z2Nat.id in Ha ; omega.
+  rewrite upd_nth_same_Zlength.
+  2,3,4: subst m' ; rewrite ?upd_nth_Zlength ?Z2Nat.id ?sub_fn_rev_s_sub_step_2_Zlength ; omega.
+  rewrite /subst_c.
+  assert(Handb:= and_0_or_1 (nth (Z.to_nat (a - 1)) m' 0 ≫ 16)).
+  assert(Handbb: Z.land (nth (Z.to_nat (a - 1)) m' 0 ≫ 16) 1 = 0 \/ Z.land (nth (Z.to_nat (a - 1)) m' 0 ≫ 16) 1 = 1) by omega.
+  clear Handb.
+  assert(- 2 ^ 16 < nth (Z.to_nat a) m' 0 ∧ nth (Z.to_nat a) m' 0 ≤ 0).
+  replace (a + 1 - 1) with a in Heqm' by omega.
+  {
+  rewrite nth_drop_2.
+  subst m'.
+  rewrite sub_fn_rev_f_skip.
+  2: rewrite Zlength_correct in H0.
+  2: omega.
+  2: omega.
+  Focus 2.
+  replace (length m')%nat with (Z.to_nat (Z.of_nat (length m')))%nat by (apply Nat2Z.id).
+  all: rewrite -Z2Nat.inj_le ; subst.
+  all: rewrite -?Zlength_correct.
+  all: rewrite ?sub_fn_rev_s_sub_step_2_Zlength ; omega.
+  rewrite -nth_drop_2.
+  Focus 2.
+  replace (length m)%nat with (Z.to_nat (Z.of_nat (length m)))%nat by (apply Nat2Z.id).
+  all: rewrite -Z2Nat.inj_le -?Zlength_correct ; omega.
+  rewrite -(nth_take_full _ (Z.to_nat 15)).
+  2: rewrite -Z2Nat.inj_lt ; omega.
+  apply Forall_nth_d.
+  compute ; split ; [reflexivity | intros; discriminate].
+  change_Z_to_nat.
+  assumption.
+  }
+  destruct Handbb as [Handbb|Handbb] ; rewrite Handbb ;  try omega.
+Qed.
+
+Local Ltac solve_this_assert :=
+  rewrite sub_fn_rev_s_n; try omega;
+  rewrite sub_step_2_Z_inv; Grind_add_Z; try assumption;
+  rewrite ?sub_fn_rev_s_sub_step_2_Zlength ; try omega;
+  apply bound_a_subst_step_2 ; auto ; omega.
+
+
+Local Ltac gen_goals P j n := match n with 
+  | 0 => idtac
+  | n => 
+    let n'' := (eval compute in (j - n)) in
+    assert(P n''); (* [admit|]; *)
+    [simpl ; solve_this_assert|];
+   let n' := (eval compute in (n - 1)) in
+   gen_goals P j n'
+  end.
+
+Lemma sub_fn_rev_s_sub_step_2_inv : forall a m,
+  0 < a < 16 ->
+  Zlength m = 16 ->
+  Forall (fun x => - 2^16 < x <= 0) (take 15 m) ->
+  ZofList 16 (sub_fn_rev_s 1 sub_step_2 a m) = ZofList 16 m.
+Proof.
+intros a m Ha Hm Hb.
+assert(Hbound: forall a, 0 < a /\ a < 16 -> - 2^16 < nth (Z.to_nat (a - 1)) m 0 <= 0).
+{
+  intros x Hx.
+  replace(nth (Z.to_nat (x - 1)) m 0) with (nth (Z.to_nat (x - 1)) (take 15 m) 0).
+  apply Forall_nth_d.
+  compute ; split ; [reflexivity | discriminate].
+  assumption.
+  apply nth_take_full.
+  change 15%nat with (Z.to_nat 15).
+  apply Z2Nat.inj_lt ; omega.
+}
+assert(H1: ℤ16.lst sub_fn_rev_s 1 sub_step_2 1 m = ℤ16.lst m).
+  rewrite sub_fn_rev_s_1 ; reflexivity.
+assert(H2: ℤ16.lst sub_fn_rev_s 1 sub_step_2 2 m = ℤ16.lst m).
+  rewrite sub_fn_rev_s_n ; try apply sub_step_2_Z_inv; [omega | | omega].
+  assert(Haspe: 0 < 2 - 1 /\ 2 - 1 < 16) by omega.
+  apply Hbound in Haspe; omega.
+gen_goals (fun x => (ℤ16.lst sub_fn_rev_s 1 sub_step_2 x m = ℤ16.lst m)) 16 13.
+assert_gen_hyp_ Hadec a 15 14 ; try omega.
+repeat match goal with
+  | _ => assumption
+  | _ => progress subst
+  | [ H : _ \/ _ |- _ ] => destruct H
+end.
+Qed.
+
+Close Scope Z.
